isabelle/Core/TimeRange.thy
@@ -2,26 +2,9 @@ theory TimeRange
 imports Semantics PositiveAccounts QuiescentResult MoneyPreservation Timeout TransactionBound
 begin
 
-
-text \<open>
-The following function checks if a closed and bounded time interval is inside 
-an open 
-\<close>
-fun inInterval :: "TimeInterval \<Rightarrow> OptBoundTimeInterval \<Rightarrow> bool" where
-"inInterval (min1, max1) (OptBoundTimeInterval (None, None)) = True" |
-"inInterval (_, max1) (OptBoundTimeInterval (None, Some max2)) = (max1 \<le> max2)" |
-"inInterval (min1, _) (OptBoundTimeInterval (Some min2, None)) = (min1 \<ge> min2)" |
-"inInterval (min1, max1) (OptBoundTimeInterval (Some min2, Some max2)) = (min1 \<ge> min2 \<and> max1 \<le> max2)"
-
-fun isCompatible :: "POSIXTime \<times> POSIXTime \<Rightarrow> POSIXTime option \<times> POSIXTime option \<Rightarrow> bool" where
-"isCompatible (min1, max1) (None, None) = True" |
-"isCompatible (_, max1) (None, Some max2) = (max1 \<le> max2)" |
-"isCompatible (min1, _) (Some min2, None) = (min1 \<ge> min2)" |
-"isCompatible (min1, max1) (Some min2, Some max2) = (min1 \<ge> min2 \<and> max1 \<le> max2)"
-
-theorem isCompatibleIdempotentToCombineInterval :
-  "isCompatible (min1, max1) (min2, max2) =
-     (combineIntervals (Some min1, Some max1) (min2, max2) = (Some min1, Some max1))"
+theorem inIntervalIdempotentToIntersectInterval :
+  "inInterval (min1, max1) (min2, max2) =
+     (intersectInterval (Bounded min1, Bounded max1) (min2, max2) = (Bounded min1, Bounded max1))"
   apply (cases min2)
   apply (cases max2)
     apply simp
@@ -34,86 +17,73 @@ theorem isCompatibleIdempotentToCombineInterval :
       by auto
     done
 
-lemma compatibleIdempotency1 :
-  "isCompatible (x, y) (combineIntervals b c) \<Longrightarrow> isCompatible (x, y) b"
+lemma inIntervalIdempotency1 :
+  "inInterval (x, y) (intersectInterval b c) \<Longrightarrow> inInterval (x, y) b"
   apply (cases b)
   apply (cases c)
   subgoal for b1 b2 c1 c2
-    apply (simp only:combineIntervals.simps)
+    apply (simp only:inInterval.simps)
     apply (cases b1)
     apply (cases c1)
-    apply (smt (verit, best) Semantics.maxOpt.simps(1) Semantics.minOpt.elims TimeRange.isCompatible.simps(1) TimeRange.isCompatible.simps(2))
-    apply (smt (verit, ccfv_threshold) Semantics.minOpt.elims TimeRange.isCompatible.simps(1) TimeRange.isCompatible.simps(2) TimeRange.isCompatible.simps(4))
+    apply (smt (verit, best) OptBoundTimeInterval.intersectInterval.simps OptBoundTimeInterval.maxLow.simps(1) OptBoundTimeInterval.minHigh.elims assoc commute inIntervalIdempotentToIntersectInterval)
+    apply (smt (verit, ccfv_threshold) OptBoundTimeInterval.inInterval.simps(2) OptBoundTimeInterval.inInterval.simps(4) OptBoundTimeInterval.intersectInterval.simps OptBoundTimeInterval.maxLow.simps(2) OptBoundTimeInterval.minHigh.elims OptBoundTimeInterval.minHigh.simps(2) inIntervalIdempotentToIntersectInterval maxLow_comm)
     apply (cases c1)
     apply simp
-    apply (smt (verit, del_insts) Option.option.sel Semantics.minOpt.elims TimeRange.isCompatible.simps(3) TimeRange.isCompatible.simps(4))
-    apply simp
-    apply (cases b2)
-    using isCompatibleIdempotentToCombineInterval apply force
-    apply (cases c2)
-     apply force
-    by simp
+    apply (smt (verit, ccfv_threshold) OptBoundTimeInterval.inInterval.simps(3) OptBoundTimeInterval.inInterval.simps(4) OptBoundTimeInterval.minHigh.elims)
+    by (smt (verit) Groups.abel_semigroup.commute Groups.semigroup.assoc OptBoundTimeInterval.intersectInterval.simps OptBoundTimeInterval.maxLow.simps(3) OptBoundTimeInterval.minHigh.elims abel_semigroup_axioms inIntervalIdempotentToIntersectInterval semigroup_axioms)
   done
 
-lemma compatibleIdempotency2 :
-  "isCompatible (x, y) (combineIntervals b c) \<Longrightarrow> isCompatible (x, y) c"
+lemma inIntervalIdempotency2 :
+  "inInterval (x, y) (intersectInterval b c) \<Longrightarrow> inInterval (x, y) c"
   apply (cases b)
   apply (cases c)
   subgoal for b1 b2 c1 c2
-    apply (simp only:combineIntervals.simps)
+    apply (simp only:intersectInterval.simps)
     apply (cases b1)
     apply (cases c1)
-    apply (smt (verit, ccfv_SIG) Semantics.maxOpt.simps(1) Semantics.minOpt.elims TimeRange.isCompatible.simps(1) TimeRange.isCompatible.simps(2))
+    apply (metis OptBoundTimeInterval.intersectInterval.simps commute inIntervalIdempotency1)
+    apply (metis OptBoundTimeInterval.intersectInterval.simps commute inIntervalIdempotency1)
     apply simp
-    apply (smt (verit, best) Semantics.minOpt.elims TimeRange.isCompatible.simps(3) TimeRange.isCompatible.simps(4))
-    apply (cases c1)
-    apply simp
-    apply (smt (verit, best) Option.option.discI Pair_inject Semantics.minOpt.elims TimeRange.isCompatible.elims(1) TimeRange.isCompatible.simps(4))
-    apply simp
-    apply (cases b2)
-    using isCompatibleIdempotentToCombineInterval apply force
-    apply (cases c2)
-     apply force
-    by simp
+    by (metis OptBoundTimeInterval.intersectInterval.simps inIntervalIdempotency1 minHigh_comm)
   done
 
 lemma compatibleIdempotencyWhen :
   "b \<le> a2 \<Longrightarrow> b \<le> a1 \<Longrightarrow>
-   isCompatible (a1, a2) (calculateTimeInterval n ct (When a b c)) \<Longrightarrow>
-   isCompatible (a1, a2) (calculateTimeInterval n ct c)"
+   inInterval (a1, a2) (calculateNonAmbiguousInterval n ct (When a b c)) \<Longrightarrow>
+   inInterval (a1, a2) (calculateNonAmbiguousInterval n ct c)"
   apply (induction a)
-  apply (smt (verit, best) Semantics.calculateTimeInterval.simps(4) TimeRange.isCompatible.simps(2) compatibleIdempotency2)
+  apply (smt (verit, best) OptBoundTimeInterval.inInterval.simps(2) Semantics.calculateNonAmbiguousInterval.simps(4) inIntervalIdempotency2)
   subgoal for c1 c2
     apply (cases c1)
     apply simp
     apply (cases "gtIfNone n 0")
      apply simp
-    using compatibleIdempotency2 apply blast
+    using inIntervalIdempotency2 apply blast
     by presburger
   done
 
-lemma calculateTimeIntervalAvoidsAmbiguousInterval_When :
-   "isCompatible (x, y) (calculateTimeInterval n ct (When a b c)) \<Longrightarrow>
+lemma calculateNonAmbiguousIntervalAvoidsAmbiguousInterval_When :
+   "inInterval (x, y) (calculateNonAmbiguousInterval n ct (When a b c)) \<Longrightarrow>
     y < b \<or> x \<ge> b"
   apply (induction a arbitrary:x y n ct b c)
   subgoal for x y n ct b c
     apply (cases "ct < b")
      apply simp
     apply auto
-    using TimeRange.isCompatible.simps(3) compatibleIdempotency1 by blast
+    using OptBoundTimeInterval.inInterval.simps(3) inIntervalIdempotency1 by blast
   subgoal for a1 a2 x y n ct b c
     apply (cases a1)
-    apply (simp only:calculateTimeInterval.simps)
+    apply (simp only:calculateNonAmbiguousInterval.simps)
     subgoal for a ac
       apply (cases "gtIfNone n 0")
        apply simp
-      using compatibleIdempotency2 apply blast
+      using inIntervalIdempotency2 apply blast
       by simp
     done
   done
 
-lemma calculateTimeIntervalAvoidsAmbiguousInterval_reduceContractStep :
-"isCompatible (timeInterval env) (calculateTimeInterval n ct contract) \<Longrightarrow>
+lemma calculateNonAmbiguousIntervalAvoidsAmbiguousInterval_reduceContractStep :
+"inInterval (timeInterval env) (calculateNonAmbiguousInterval n ct contract) \<Longrightarrow>
  reduceContractStep env state contract \<noteq> AmbiguousTimeIntervalReductionError"
   apply (cases contract)
   apply (cases "refundOne (accounts state)")
@@ -125,21 +95,21 @@ lemma calculateTimeIntervalAvoidsAmbiguousInterval_reduceContractStep :
   subgoal for a b c
     apply (auto split:prod.splits)
     subgoal for x y
-      using calculateTimeIntervalAvoidsAmbiguousInterval_When by blast
+      using calculateNonAmbiguousIntervalAvoidsAmbiguousInterval_When by blast
     done
   apply (simp add:Let_def)
   by simp
 
 lemma resultOfReduceIsCompatibleToo :
-  "isCompatible (timeInterval env) (calculateTimeInterval n ct contract) \<Longrightarrow>
+  "inInterval (timeInterval env) (calculateNonAmbiguousInterval n ct contract) \<Longrightarrow>
    reduceContractStep env state contract = Reduced x11 x12 x13 x14 \<Longrightarrow>
-   isCompatible (timeInterval env) (calculateTimeInterval n ct x14)"
+   inInterval (timeInterval env) (calculateNonAmbiguousInterval n ct x14)"
   apply (cases contract)
   using reduceStepClose_is_Close apply blast
   subgoal for a b c d e
     apply (cases "evalValue env state d \<le> 0")
     by (simp_all add:Let_def)
-     apply (smt (verit, best) Semantics.ReduceStepResult.inject Semantics.calculateTimeInterval.simps(3) Semantics.reduceContractStep.simps(3) TimeRange.isCompatible.elims(2) compatibleIdempotency1 compatibleIdempotency2)
+    apply (smt (verit, del_insts) OptBoundTimeInterval.inInterval.elims(3) Semantics.ReduceStepResult.inject Semantics.calculateNonAmbiguousInterval.simps(3) Semantics.reduceContractStep.simps(3) inIntervalIdempotency1 inIntervalIdempotency2)
   subgoal for a b c
     apply (cases "timeInterval env")
     apply (simp only:reduceContractStep.simps Let_def prod.case)
@@ -152,14 +122,14 @@ lemma resultOfReduceIsCompatibleToo :
        apply (meson compatibleIdempotencyWhen linorder_not_le)
       by simp
     done
-  apply (metis Semantics.ReduceStepResult.inject Semantics.calculateTimeInterval.simps(6) Semantics.reduceContractStep.simps(5))
+  apply (metis Semantics.ReduceStepResult.inject Semantics.calculateNonAmbiguousInterval.simps(6) Semantics.reduceContractStep.simps(5))
   by simp
 
 
 lemma resultOfReductionLoopQuiescentIsCompatibleToo :
-  "isCompatible (timeInterval env) (calculateTimeInterval n ct contract) \<Longrightarrow>
+  "inInterval (timeInterval env) (calculateNonAmbiguousInterval n ct contract) \<Longrightarrow>
    reductionLoop b env state contract wa ef = ContractQuiescent x11 x12 x13 x14 x15 \<Longrightarrow>
-   isCompatible (timeInterval env) (calculateTimeInterval n ct x15)"
+   inInterval (timeInterval env) (calculateNonAmbiguousInterval n ct x15)"
   apply (induction b env state contract wa ef rule:reductionLoop.induct)
   subgoal for reduced env state contract warnings payments
     apply (simp only:reductionLoop.simps[of reduced env state contract warnings payments])
@@ -172,13 +142,13 @@ lemma resultOfReductionLoopQuiescentIsCompatibleToo :
   done
 
 lemma resultOfReduceUntilQuiescentIsCompatibleToo :
-  "isCompatible (timeInterval env) (calculateTimeInterval n ct contract) \<Longrightarrow>
+  "inInterval (timeInterval env) (calculateNonAmbiguousInterval n ct contract) \<Longrightarrow>
    reduceContractUntilQuiescent env state contract = ContractQuiescent x11 x12 x13 x14 x15 \<Longrightarrow>
-   isCompatible (timeInterval env) (calculateTimeInterval n ct x15)"
+   inInterval (timeInterval env) (calculateNonAmbiguousInterval n ct x15)"
   by (metis Semantics.reduceContractUntilQuiescent.simps resultOfReductionLoopQuiescentIsCompatibleToo)
 
-lemma calculateTimeIntervalAvoidsAmbiguousInterval_reduceContractUntilQuiescent :
-"isCompatible (timeInterval env) (calculateTimeInterval n ct contract) \<Longrightarrow>
+lemma calculateNonAmbiguousIntervalAvoidsAmbiguousInterval_reduceContractUntilQuiescent :
+"inInterval (timeInterval env) (calculateNonAmbiguousInterval n ct contract) \<Longrightarrow>
  reductionLoop b env state contract wa err \<noteq> RRAmbiguousTimeIntervalError"
   apply (induction b env state contract wa err rule:reductionLoop.induct)
   subgoal for reduced env state contract warnings payments
@@ -187,7 +157,7 @@ lemma calculateTimeIntervalAvoidsAmbiguousInterval_reduceContractUntilQuiescent 
       apply (simp only:ReduceStepResult.case Let_def)
     using resultOfReduceIsCompatibleToo apply presburger
      apply simp
-    using calculateTimeIntervalAvoidsAmbiguousInterval_reduceContractStep by auto
+    using calculateNonAmbiguousIntervalAvoidsAmbiguousInterval_reduceContractStep by auto
   done
 
 fun childCase :: "Contract \<Rightarrow> Case list \<Rightarrow> bool" where
@@ -223,23 +193,23 @@ lemma successInApplyCasesReturnChildCase :
   done
 
 lemma resultOfApplyCaseIsCompatibleToo_aux :
-"isCompatible (timeInterval env) (calculateTimeInterval n ct (When x41 x42 x43)) \<Longrightarrow>
+"inInterval (timeInterval env) (calculateNonAmbiguousInterval n ct (When x41 x42 x43)) \<Longrightarrow>
  childCase ncont x41 \<Longrightarrow> ct < x42 \<Longrightarrow> gtIfNone n 0 \<Longrightarrow>
- isCompatible (timeInterval env) (calculateTimeInterval (subIfSome n 1) ct ncont)"
+ inInterval (timeInterval env) (calculateNonAmbiguousInterval (subIfSome n 1) ct ncont)"
   apply (induction x41)
    apply simp
   subgoal for h t
     apply (cases h)
     subgoal for x y
       apply simp
-    by (smt (verit, best) TimeRange.isCompatible.elims(3) compatibleIdempotency1 compatibleIdempotency2)
+      by (smt (verit, best) OptBoundTimeInterval.inInterval.elims(3) inIntervalIdempotency1 inIntervalIdempotency2)
   done
   done
 
 lemma resultOfApplyCaseIsCompatibleToo :
-"isCompatible (timeInterval env) (calculateTimeInterval n ct (When x41 x42 x43)) \<Longrightarrow>
+"inInterval (timeInterval env) (calculateNonAmbiguousInterval n ct (When x41 x42 x43)) \<Longrightarrow>
  applyCases env sta h x41 = Applied nwa nsta ncont \<Longrightarrow> ct < x42 \<Longrightarrow> gtIfNone n 0 \<Longrightarrow>
- isCompatible (timeInterval env) (calculateTimeInterval (subIfSome n 1) ct ncont)"
+ inInterval (timeInterval env) (calculateNonAmbiguousInterval (subIfSome n 1) ct ncont)"
   by (simp add: resultOfApplyCaseIsCompatibleToo_aux successInApplyCasesReturnChildCase)
 
 fun ifCaseLt :: "POSIXTime \<Rightarrow> Contract \<Rightarrow> bool" where
@@ -247,9 +217,9 @@ fun ifCaseLt :: "POSIXTime \<Rightarrow> Contract \<Rightarrow> bool" where
 "ifCaseLt _ _ = True"
 
 lemma resultOfApplyInputIsCompatibleToo :
-"isCompatible (timeInterval env) (calculateTimeInterval n ct cont) \<Longrightarrow>
+"inInterval (timeInterval env) (calculateNonAmbiguousInterval n ct cont) \<Longrightarrow>
  applyInput env sta h cont = Applied nwa nsta ncont \<Longrightarrow> ifCaseLt ct cont \<Longrightarrow> gtIfNone n 0 \<Longrightarrow>
- isCompatible (timeInterval env) (calculateTimeInterval (subIfSome n 1) ct ncont)"
+ inInterval (timeInterval env) (calculateNonAmbiguousInterval (subIfSome n 1) ct ncont)"
   apply (cases cont)
   apply simp_all
   by (simp add: resultOfApplyCaseIsCompatibleToo)
@@ -261,19 +231,19 @@ lemma geIfNone_redListSize :
 fun isValidInterval :: "POSIXTime \<times> POSIXTime \<Rightarrow> bool" where
 "isValidInterval (a, b) = (a \<le> b)"
 
-lemma reduceStep_ifCaseLtCt_aux : "isCompatible (a, b) (calculateTimeInterval n ct (When x41 x42 x43)) \<Longrightarrow>
+lemma reduceStep_ifCaseLtCt_aux : "inInterval (a, b) (calculateNonAmbiguousInterval n ct (When x41 x42 x43)) \<Longrightarrow>
                                    a \<le> b \<Longrightarrow> env = \<lparr>timeInterval = (a, b)\<rparr> \<Longrightarrow> b < x42 \<Longrightarrow> ct < x42"
   apply (induction x41)
    apply simp
-   apply (smt (verit, best) TimeRange.isCompatible.simps(3) compatibleIdempotency1)
+   apply (smt (verit, best) OptBoundTimeInterval.inInterval.simps(3) inIntervalIdempotency1)
   subgoal for h t
     apply simp
     apply (cases h)
     apply simp
-  using compatibleIdempotency2 by presburger
+  using inIntervalIdempotency2 by presburger
   done
 
-lemma reduceStep_ifCaseLtCt : "isCompatible (timeInterval env) (calculateTimeInterval n ct (When x41 x42 x43)) \<Longrightarrow>
+lemma reduceStep_ifCaseLtCt : "inInterval (timeInterval env) (calculateNonAmbiguousInterval n ct (When x41 x42 x43)) \<Longrightarrow>
                                reduceContractStep env state (When x41 x42 x43) = NotReduced \<Longrightarrow> isValidInterval (timeInterval env) \<Longrightarrow> ct < x42"
   apply (cases env)
   subgoal for timeInterv
@@ -288,7 +258,7 @@ lemma reduceStep_ifCaseLtCt : "isCompatible (timeInterval env) (calculateTimeInt
   done
 
 
-lemma reduceLoop_ifCaseLtCt : "isCompatible (timeInterval env) (calculateTimeInterval n ct cont) \<Longrightarrow>
+lemma reduceLoop_ifCaseLtCt : "inInterval (timeInterval env) (calculateNonAmbiguousInterval n ct cont) \<Longrightarrow>
                                reductionLoop b env state cont wa ef = ContractQuiescent x11 x12 x13 x14 x15 \<Longrightarrow> isValidInterval (timeInterval env) \<Longrightarrow> ifCaseLt ct x15"
   apply (induction b env state cont wa ef rule:reductionLoop.induct)
   subgoal for reduced env state contract warnings payments
@@ -309,15 +279,15 @@ lemma reduceLoop_ifCaseLtCt : "isCompatible (timeInterval env) (calculateTimeInt
     using TimeRange.ifCaseLt.simps(6) by blast
   done
 
-lemma reduceContractUntilQuiescent_ifCaseLtCt : "isCompatible (timeInterval env) (calculateTimeInterval n ct cont) \<Longrightarrow>
+lemma reduceContractUntilQuiescent_ifCaseLtCt : "inInterval (timeInterval env) (calculateNonAmbiguousInterval n ct cont) \<Longrightarrow>
                                                  reduceContractUntilQuiescent env state cont = ContractQuiescent x11 x12 x13 x14 x15 \<Longrightarrow>
                                                  isValidInterval (timeInterval env) \<Longrightarrow> ifCaseLt ct x15"
   apply (simp only:reduceContractUntilQuiescent.simps)
   by (simp add: reduceLoop_ifCaseLtCt)
 
-lemma calculateTimeIntervalAvoidsAmbiguousInterval_applyAllLoop :
+lemma calculateNonAmbiguousIntervalAvoidsAmbiguousInterval_applyAllLoop :
 "geIfNone n (int (length inps)) \<Longrightarrow>
- isCompatible (timeInterval env) (calculateTimeInterval n ct c) \<Longrightarrow>
+ inInterval (timeInterval env) (calculateNonAmbiguousInterval n ct c) \<Longrightarrow>
  isValidInterval (timeInterval env) \<Longrightarrow>
  applyAllLoop b env s c inps wa ef \<noteq>
  ApplyAllAmbiguousTimeIntervalError"
@@ -346,21 +316,21 @@ lemma calculateTimeIntervalAvoidsAmbiguousInterval_applyAllLoop :
             using Semantics.gtIfNone.elims(3) fact(2) of_nat_le_iff by fastforce
           done
         by (metis Semantics.ApplyAllResult.distinct(5) Semantics.ApplyResult.simps(5))
-      using calculateTimeIntervalAvoidsAmbiguousInterval_reduceContractUntilQuiescent by auto
+      using calculateNonAmbiguousIntervalAvoidsAmbiguousInterval_reduceContractUntilQuiescent by auto
     done
 
-lemma calculateTimeIntervalAvoidsAmbiguousInterval_applyAllInputs :
+lemma calculateNonAmbiguousIntervalAvoidsAmbiguousInterval_applyAllInputs :
 "geIfNone n (int (length inps)) \<Longrightarrow>
- isCompatible (minInterv, maxInterv) (calculateTimeInterval n ct c) \<Longrightarrow>
+ inInterval (minInterv, maxInterv) (calculateNonAmbiguousInterval n ct c) \<Longrightarrow>
  isValidInterval (minInterv, maxInterv) \<Longrightarrow>
  applyAllInputs \<lparr> timeInterval = (minInterv, maxInterv) \<rparr> s c inps
     \<noteq> ApplyAllAmbiguousTimeIntervalError"
   apply (simp only:applyAllInputs.simps)
-  using calculateTimeIntervalAvoidsAmbiguousInterval_applyAllLoop by auto
+  using calculateNonAmbiguousIntervalAvoidsAmbiguousInterval_applyAllLoop by auto
 
-theorem calculateTimeIntervalAvoidsAmbiguousInterval :
+theorem calculateNonAmbiguousIntervalAvoidsAmbiguousInterval :
   "geIfNone n (int (length (inputs tx))) \<Longrightarrow>
-   isCompatible (interval tx) (calculateTimeInterval n ct c) \<Longrightarrow>
+   inInterval (interval tx) (calculateNonAmbiguousInterval n ct c) \<Longrightarrow>
    computeTransaction tx s c \<noteq> TransactionError TEAmbiguousTimeIntervalError"
   apply (simp only:computeTransaction.simps Let_def)
   apply (cases tx)
@@ -371,9 +341,28 @@ theorem calculateTimeIntervalAvoidsAmbiguousInterval :
       apply (cases "applyAllInputs \<lparr>timeInterval = (max minInterv (minTime s), maxInterv)\<rparr>
            (s\<lparr>minTime := max minInterv (minTime s)\<rparr>) c inps")
       apply simp
-      apply simp
+       apply simp
       apply (simp del:applyAllInputs.simps)
-      by (smt (verit) Semantics.applyAllInputs.simps SemanticsTypes.Environment.select_convs(1) TimeRange.isCompatible.elims(2) TimeRange.isCompatible.simps(1) TimeRange.isCompatible.simps(2) TimeRange.isCompatible.simps(3) TimeRange.isCompatible.simps(4) TimeRange.isValidInterval.simps calculateTimeIntervalAvoidsAmbiguousInterval_applyAllLoop)
+      apply (cases s)
+      apply (simp del:applyAllInputs.simps)
+      subgoal for accounts choices boundValues minTime
+        apply (cases "minInterv \<le> minTime")
+        apply (simp del:applyAllInputs.simps)
+         apply (smt (verit, ccfv_threshold) OptBoundTimeInterval.inInterval.elims(3) OptBoundTimeInterval.inInterval.simps(2) OptBoundTimeInterval.inInterval.simps(3) OptBoundTimeInterval.inInterval.simps(4) TimeRange.isValidInterval.simps calculateNonAmbiguousIntervalAvoidsAmbiguousInterval_applyAllInputs)
+        by (metis Lattices.linorder_class.max.absorb4 Lattices.linorder_class.max.commute TimeRange.isValidInterval.simps calculateNonAmbiguousIntervalAvoidsAmbiguousInterval_applyAllInputs linorder_not_le)
+      done
     done
   done
+
+corollary calculateNonAmbiguousIntervalAvoidsAmbiguousInterval_bounded :
+  "n \<ge> (int (length (inputs tx))) \<Longrightarrow>
+   inInterval (interval tx) (calculateNonAmbiguousInterval (Some n) ct c) \<Longrightarrow>
+   computeTransaction tx s c \<noteq> TransactionError TEAmbiguousTimeIntervalError"
+  using Semantics.geIfNone.simps(2) calculateNonAmbiguousIntervalAvoidsAmbiguousInterval by blast
+
+corollary calculateNonAmbiguousIntervalAvoidsAmbiguousInterval_unbounded :
+  "inInterval (interval tx) (calculateNonAmbiguousInterval None ct c) \<Longrightarrow>
+   computeTransaction tx s c \<noteq> TransactionError TEAmbiguousTimeIntervalError"
+  by (meson Semantics.geIfNone.simps(1) calculateNonAmbiguousIntervalAvoidsAmbiguousInterval)
+
 end
